

Items I , $i \in I$

Features F , $f \in F$

Nodes N , $j \in N$

l_j : j is a leaf

v_{ij} : Item i is valid at node j

S_{jf} : Node j discriminates on feature f

t_j : Value for node j

σ_{fi} The value of feature f in item i

d_{fj}^0 If 1, Node j discriminates on feature f and the feature value is 0 exist at least one item's value of the same feature is 0

d_{fj}^1 If 1, Node j discriminates on feature f and the feature value is 1 exist at least one item's value of the same feature is 1

vd_{ij} If 1, item i is valid at decision node J and has the same feature value as the feature value at node J

vl_{ij} If 1, item i is valide at the leaf node J

c_i The class value of item i

$$(1) \quad \bigvee_{i \in I} v_{i1} = 1$$

$$v_{i1} \wedge v_{21} \wedge v_{31} \cdots \wedge v_{i1}$$

(2)

$$(2A) \quad d_{fj}^0 \leftrightarrow S_{jf} \wedge \neg t_j \quad \text{When } \sigma_{fi} = 0$$

$$(\neg d_{fj}^0 \vee S_{jf}) \wedge (\neg d_{fj}^0 \vee \neg t_j) \wedge (d_{fj}^0 \vee \neg S_{jf} \vee t_j)$$

$$(2B) \quad d_{fj}^1 \leftrightarrow S_{jf} \wedge t_j \quad \text{When } \sigma_{fi} = 1$$

$$(\neg d_{fj}^1 \vee S_{jf}) \wedge (\neg d_{fj}^1 \vee t_j) \wedge (d_{fj}^1 \vee \neg S_{jf} \vee \neg t_j)$$

$$(33) \quad vd_{ij} \leftrightarrow v_{ij} \wedge \bigvee_{f \in F} d_{fj}^{\sigma_{fi}}$$

$$A \leftrightarrow B \wedge C$$

$$(\neg A \vee B) \wedge (\neg B \vee C) \wedge (A \vee \neg B \vee \neg C)$$

$$(\neg A \vee B) \wedge (\neg B \vee d_{1j} \vee d_{2j} \cdots \vee d_{fj}) \wedge (A \vee \neg B \vee \neg d_{1j}) \wedge (A \vee \neg B \vee \neg d_{2j}) \cdots \wedge (A \vee \neg B \vee \neg d_{fj})$$

$$(\neg vd_{ij} \vee v_{ij}) \wedge (\neg v_{ij} \vee d_{1j} \vee d_{2j} \cdots \vee d_{fj}) \wedge (vd_{ij} \vee \neg v_{ij} \vee \neg d_{1j}) \wedge (vd_{ij} \vee \neg v_{ij} \vee \neg d_{2j}) \cdots \wedge (vd_{ij} \vee \neg v_{ij} \vee \neg d_{fj})$$

$$(44) \quad \bigvee_{i,j \in I, 1..N-1} v_{i(j+1)} \leftrightarrow l_j \vee vd_{ij} \quad |I||N||F|$$

$$A \leftrightarrow B \vee C$$

$$(\neg A \vee B \vee C) \wedge (A \vee \neg B) \wedge (A \vee \neg C)$$

$$(\neg v_{i(j+1)} \vee l_j \vee vd_{ij}) \wedge (v_{i(j+1)} \vee \neg l_j) \wedge (v_{i(j+1)} \vee \neg vd_{ij})$$

$$(55) \quad \bigvee_{j \in N} \sum_{f \in F} S_{jf} + l_j = 1 \quad |N||F|$$

$$(55a) \quad l_j \leftrightarrow \bigvee_{f \in F} \neg S_{jf}$$

$$(\neg l_j \vee \neg S_{j1}) \wedge (l_j \vee S_{j1}) \wedge (\neg l_j \vee \neg S_{j2}) \wedge (l_j \vee S_{j2}) \cdots \wedge (\neg l_j \vee \neg S_{jf}) \wedge (l_j \vee S_{jf})$$

$$(55b) \quad \bigvee_{j \in N} \sum_{f \in F} (S_{jf} \vee l_j) = 1 \quad |N||F|$$

$$(6) \quad S_{(j+1)f} \rightarrow l_j \vee \bigvee_{f' < f} S_{jf'} \quad |N-2||F|$$

$$\neg A \vee B \vee C$$

$$\neg S_{(j+1)f} \vee l_j \vee \bigvee_{f' < f} S_{jf'}$$

(7) $vl_{ij} \leftrightarrow l_j \wedge v_{ij}$

$(\neg vl_{ij} \vee l_j) \wedge (\neg vl_{ij} \vee v_{ij}) \wedge (vl_{ij} \vee \neg l_j \vee \neg v_{ij})$

(8) $\bigvee_{i \in I} \sum_{j \in N} vl_{ij} = 1 \quad |N| \mid |I|$

(9) $\bigvee_{i \in I} \bigvee_{j \in J} vl_{ij} \rightarrow c_i = t_j \quad |N| \mid |I|$

$\neg A \vee B$

(2XX) $S_{jf} \rightarrow \bigvee_{i \in I} (\sigma_{fi} = t_j) \quad f \in F$

(3XX) $\bigvee_{i,j \in I, 1..N-1} v_{i(j+1)} = l_j \vee (v_{ij} \wedge S_{jf}) \quad |I| \mid |N| \mid |F|$